SpecFuns now compiles (again).

LambdaS5/coq/LjsRulesCorrectDefinitions.v
@@ -192,21 +192,12 @@ Inductive option_value_related BR : option J.value -> option L.value -> Prop :=
     option_value_related BR (Some jv) (Some v)
 .
 
-Inductive primval_related BR : option J.value -> L.object -> Prop :=
-| primval_related_none : forall obj, 
-    ~index (L.object_internal obj) "primval" -> 
-    primval_related BR None obj
-| primval_related_some : forall obj jv v, 
-    binds (L.object_internal obj) "primval" v ->
-    value_related BR jv v ->
-    primval_related BR (Some jv) obj
-.
-
 Record object_prim_related BR jobj obj : Prop := {
     object_prim_related_class : J.object_class_ jobj = L.object_class obj;
     object_prim_related_extensible : J.object_extensible_ jobj = L.object_extensible obj;
     object_prim_related_prototype : value_related BR (J.object_proto_ jobj) (L.object_proto obj);
-    object_prim_related_primval : primval_related BR (J.object_prim_value_ jobj) obj
+    object_prim_related_primval : 
+        option_value_related BR (J.object_prim_value_ jobj) (L.object_internal obj\("primval"?))
 }.
 
 Record object_related BR jobj obj : Prop := {
@@ -461,6 +452,12 @@ Record env_records_exist BR jc := {
     States that EcmaScript preallocated objects can be found in the LJS context. *)
 
 Definition prealloc_in_ctx_list := [
+    (J.prealloc_global, "%global");
+    (J.prealloc_global_eval, "%global");
+    (J.prealloc_global_is_finite, "%isFinite");
+    (J.prealloc_global_is_nan, "%isNaN");
+    (J.prealloc_global_parse_float, "%parseFloat");
+    (J.prealloc_global_parse_int, "%parseInt");
     (J.prealloc_native_error J.native_error_eval, "%EvalErrorGlobalFuncObj");
     (J.prealloc_native_error J.native_error_range, "%RangeErrorGlobalFuncObj");
     (J.prealloc_native_error J.native_error_ref, "%ReferenceErrorGlobalFuncObj");
@@ -470,7 +467,26 @@ Definition prealloc_in_ctx_list := [
     (J.prealloc_native_error_proto J.native_error_range, "%RangeErrorProto");
     (J.prealloc_native_error_proto J.native_error_ref, "%ReferenceErrorProto");
     (J.prealloc_native_error_proto J.native_error_syntax, "%SyntaxErrorProto");
-    (J.prealloc_native_error_proto J.native_error_type, "%TypeErrorProto")
+    (J.prealloc_native_error_proto J.native_error_type, "%TypeErrorProto");
+    (J.prealloc_object, "%ObjectGlobalFuncObj");
+    (J.prealloc_object_proto, "%ObjectProto");
+    (J.prealloc_object_proto_to_string, "%objectToString");
+    (J.prealloc_function, "%FunctionGlobalFuncObj");
+    (J.prealloc_function_proto, "%FunctionProto");
+    (J.prealloc_function_proto_to_string, "%functionToString");
+    (J.prealloc_bool, "%BooleanGlobalFuncObj");
+    (J.prealloc_bool_proto, "%BooleanProto");
+    (J.prealloc_bool_proto_to_string, "%booleanToString");
+    (J.prealloc_number, "%NumberGlobalFuncObj");
+    (J.prealloc_number_proto, "%NumberProto");
+    (J.prealloc_number_proto_to_string, "%numberToString");
+    (J.prealloc_string, "%StringGlobalFuncObj");
+    (J.prealloc_string_proto, "%StringProto");
+    (J.prealloc_string_proto_to_string, "%stringToString");
+    (J.prealloc_array, "%ArrayGlobalFuncObj");
+    (J.prealloc_array_proto, "%ArrayProto");
+    (J.prealloc_array_proto_to_string, "%arrayToString");
+    (J.prealloc_math, "%Math")
 ].
 
 Definition prealloc_in_ctx BR c := forall jpre s v, 
@@ -510,23 +526,18 @@ Parameter initBR : fact_set. (* TODO *)
 (** *** Invariant predicate
     The complete set of invariants, combined in one predicate to make proofs simpler. *)
 
-Record state_invariant BR jst jc c st : Prop := {
-    state_invariant_bisim_includes_init : initBR \c BR;
+Record state_invariant BR jst st : Prop := {
     state_invariant_heaps_bisim_consistent : heaps_bisim_consistent BR jst st;
     state_invariant_ctx_parent_ok : ctx_parent_ok BR st;
     state_invariant_getter_proxy_ok : getter_proxy_ok BR st;
     state_invariant_setter_proxy_ok : setter_proxy_ok BR st;
-    state_invariant_execution_ctx_related : execution_ctx_related BR jc c;
-    state_invariant_includes_init_ctx : includes_init_ctx c;
-    state_invariant_env_records_exist : env_records_exist BR jc;
-    state_invariant_prealloc_related : prealloc_in_ctx BR c;
-    state_invariant_global_env_record_exists : global_env_record_exists BR c;
     state_invariant_js_state_fresh_ok : J.state_fresh_ok jst
 }.
 
 (** *** For restoring invariants after function application *)
 
 Record context_invariant BR jc c : Prop := {
+    context_invariant_bisim_includes_init : initBR \c BR;
     context_invariant_execution_ctx_related : execution_ctx_related BR jc c;
     context_invariant_includes_init_ctx : includes_init_ctx c;
     context_invariant_env_records_exist : env_records_exist BR jc;
@@ -545,7 +556,7 @@ Definition concl_ext_expr_value BR jst jc c st st' r jee P :=
     J.red_expr jst jc jee (J.out_ter jst' jr) /\ 
     ((exists jv, jr = J.res_val jv /\ P jv) \/
      J.abort (J.out_ter jst' jr) /\ J.res_type jr = J.restype_throw) /\
-    state_invariant BR' jst' jc c st' /\
+    state_invariant BR' jst' st' /\
     BR \c BR' /\
     res_related BR' jst' st' jr r.
 
@@ -556,20 +567,20 @@ Definition concl_expr_value BR jst jc c st st' r je :=
 Definition concl_stat BR jst jc c st st' r jt :=
     exists BR' jst' jr,
     J.red_stat jst jc (J.stat_basic jt) (J.out_ter jst' jr) /\ 
-    state_invariant BR' jst' jc c st' /\
+    state_invariant BR' jst' st' /\
     BR \c BR' /\
     res_related BR' jst' st' jr r.
 
 Definition concl_spec {A : Type} BR jst jc c st st' r jes 
     (P : fact_set -> J.state -> A -> Prop) :=
     exists BR' jst' sr,
-    J.red_spec jst jc jes sr ->
+    J.red_spec jst jc jes sr /\
     ((exists x, sr = J.specret_val jst' x /\ P BR' jst' x) \/
      (exists jr, sr = @J.specret_out A (J.out_ter jst' jr) /\ 
         J.abort (J.out_ter jst' jr) /\ 
         J.res_type jr = J.restype_throw /\
         res_related BR' jst' st' jr r)) /\
-    state_invariant BR' jst' jc c st' /\ 
+    state_invariant BR' jst' st' /\ 
     BR \c BR'.
 
 Definition concl_expr_getvalue BR jst jc c st st' r je := 
@@ -579,32 +590,37 @@ Definition concl_expr_getvalue BR jst jc c st st' r je :=
 (** *** Theorem statements *)
 
 Definition th_expr k je := forall BR jst jc c st st' r, 
-    state_invariant BR jst jc c st ->
+    context_invariant BR jc c ->
+    state_invariant BR jst st ->
     L.red_exprh k c st (L.expr_basic (js_expr_to_ljs je)) (L.out_ter st' r) ->
     concl_expr_getvalue BR jst jc c st st' r je.
 
 Definition th_stat k jt := forall BR jst jc c st st' r, 
-    state_invariant BR jst jc c st ->
+    context_invariant BR jc c ->
+    state_invariant BR jst st ->
     L.red_exprh k c st (L.expr_basic (js_stat_to_ljs jt)) (L.out_ter st' r) ->
     concl_stat BR jst jc c st st' r jt.
 
 Definition th_spec {A : Type} k e jes 
     (P : fact_set -> J.state -> J.execution_ctx -> L.ctx -> L.store -> L.res -> A -> Prop) := 
     forall BR jst jc c st st' r, 
-    state_invariant BR jst jc c st ->
+    context_invariant BR jc c ->
+    state_invariant BR jst st ->
     L.red_exprh k c st (L.expr_basic e) (L.out_ter st' r) ->
     concl_spec BR jst jc c st st' r jes (fun BR' jst' a => P BR' jst' jc c st' r a).
 
 Definition th_ext_expr_unary k v jeef P :=
     forall BR jst jc c st st' r v1 jv1, 
-    state_invariant BR jst jc c st ->
+    context_invariant BR jc c ->
+    state_invariant BR jst st ->
     value_related BR jv1 v1 -> 
     L.red_exprh k c st (L.expr_app_2 v [v1]) (L.out_ter st' r) ->
     concl_ext_expr_value BR jst jc c st st' r (jeef jv1) P.
 
 Definition th_ext_expr_binary k v jeef P :=
     forall BR jst jc c st st' r v1 jv1 v2 jv2, 
-    state_invariant BR jst jc c st ->
+    context_invariant BR jc c ->
+    state_invariant BR jst st ->
     value_related BR jv1 v1 -> 
     value_related BR jv2 v2 -> 
     L.red_exprh k c st (L.expr_app_2 v [v1; v2]) (L.out_ter st' r) ->
